feat: upstream definition of Vector from Batteries (#6197)
This PR upstreams the definition of `Vector` from Batteries, along with
the basic functions.

tests/lean/1081.lean
@@ -10,28 +10,28 @@ example : f 0 0 = 0 := rfl
 
 example : f 0 (y+1) = y+1 := rfl
 
-inductive Vector (α : Type u) : Nat → Type u where
-  | nil  : Vector α 0
-  | cons : α → Vector α n → Vector α (n+1)
+inductive Vector' (α : Type u) : Nat → Type u where
+  | nil  : Vector' α 0
+  | cons : α → Vector' α n → Vector' α (n+1)
 
-namespace Vector
-  def insert (a: α): Fin (n+1) → Vector α n → Vector α (n+1)
+namespace Vector'
+  def insert (a: α): Fin (n+1) → Vector' α n → Vector' α (n+1)
   | ⟨0  , _⟩,        xs => cons a   xs
   | ⟨i+1, h⟩, cons x xs => cons x $ xs.insert a ⟨i, Nat.lt_of_succ_lt_succ h⟩
 
-  theorem insert_at_0_eq_cons1 (a: α) (v: Vector α n):  v.insert a ⟨0, Nat.zero_lt_succ n⟩ = cons a v :=
+  theorem insert_at_0_eq_cons1 (a: α) (v: Vector' α n):  v.insert a ⟨0, Nat.zero_lt_succ n⟩ = cons a v :=
     rfl -- Error, it does not hold by reflexivity because the recursion is on v
 
   example (a : α) :  nil.insert a ⟨0, by simp_arith⟩ = cons a nil :=
     rfl
 
-  example (a : α) (b : α) (bs : Vector α n) :  (cons b bs).insert a ⟨0, by simp_arith⟩ = cons a (cons b bs) :=
+  example (a : α) (b : α) (bs : Vector' α n) :  (cons b bs).insert a ⟨0, by simp_arith⟩ = cons a (cons b bs) :=
     rfl
 
-  theorem insert_at_0_eq_cons2 (a: α) (v: Vector α n):  v.insert a ⟨0, Nat.zero_lt_succ n⟩ = cons a v := by
+  theorem insert_at_0_eq_cons2 (a: α) (v: Vector' α n):  v.insert a ⟨0, Nat.zero_lt_succ n⟩ = cons a v := by
     rw [insert]
 
-  theorem insert_at_0_eq_cons3 (a: α) (v: Vector α n):  v.insert a ⟨0, Nat.zero_lt_succ n⟩ = cons a v := by
+  theorem insert_at_0_eq_cons3 (a: α) (v: Vector' α n):  v.insert a ⟨0, Nat.zero_lt_succ n⟩ = cons a v := by
     simp only [insert]
 
-end Vector
+end Vector'
