tests/lean/run/1024.lean
@@ -1,17 +1,17 @@
-inductive Vector (α : Type u): Nat → Type u where
-| nil : Vector α 0
-| cons (head : α) (tail : Vector α n) : Vector α (n+1)
+inductive Vector' (α : Type u): Nat → Type u where
+| nil : Vector' α 0
+| cons (head : α) (tail : Vector' α n) : Vector' α (n+1)
 
-namespace Vector
-  def nth : ∀{n}, Vector α n → Fin n → α
+namespace Vector'
+  def nth : ∀{n}, Vector' α n → Fin n → α
   | n+1, cons x xs, ⟨  0, _⟩ => x
   | n+1, cons x xs, ⟨k+1, h⟩ => xs.nth ⟨k, sorry⟩
 
-  def snoc : ∀{n : Nat} (xs : Vector α n) (x : α), Vector α (n+1)
+  def snoc : ∀{n : Nat} (xs : Vector' α n) (x : α), Vector' α (n+1)
   | _, nil,    x' => cons x' nil
   | _, cons x xs, x' => cons x (snoc xs x')
 
-  theorem nth_snoc_eq (k: Fin (n+1))(v : Vector α n)
+  theorem nth_snoc_eq (k: Fin (n+1))(v : Vector' α n)
     (h: k.val = n):
     (v.snoc x).nth k = x := by
     cases k; rename_i k hk
@@ -19,11 +19,11 @@ namespace Vector
     · simp only [nth]
     · simp! [*]
 
-  theorem nth_snoc_eq_works (k: Fin (n+1))(v : Vector α n)
+  theorem nth_snoc_eq_works (k: Fin (n+1))(v : Vector' α n)
     (h: k.val = n):
     (v.snoc x).nth k = x := by
     cases k; rename_i k hk
     induction v generalizing k <;> subst h
     · simp only [nth]
     · simp[*,nth]
-end Vector
+end Vector'
